Correction v2

core_c/operations_term.v
@@ -6,10 +6,10 @@ Local Open Scope ctype_scope.
 Local Open Scope Z_scope.
 Local Open Scope int_type_scope.
 Local Coercion Z.of_nat: nat >-> Z.
-
 Section operations_definitions2.
+  
   Context `{Env K}.
-  (* ACSL values *)
+  (*Definition of miniACSL values*)
   Inductive val_term (K : iType) : iType :=
   | ValC : val K -> val_term K
   | VInteger : Z -> val_term K.
@@ -17,23 +17,25 @@ Section operations_definitions2.
   Arguments ValC {_} _.
   Arguments VInteger {_} _.
   
-  (* Underspecified constructor for division by zero *)
+
+  (* Divide by zero :  under-specified term *)
   Parameter divZ : Z -> Z.
   
-  
+  (*miniACSL binary operations*)
   Inductive tbinop :=
   | TArithOp : arithop -> tbinop
   | TShiftOp : shiftop -> tbinop
   | TBitOp : bitop -> tbinop.
-  
+
+  (*Conversion from miniACSL binary operation to C binary operation*)
   Definition tbin_to_bin (op : tbinop):=
     match op with
     | TArithOp opa => ArithOp opa
     | TShiftOp ops => ShiftOp ops 
     | TBitOp opb => BitOp opb
     end.
-  
-  (* Arithop for integers with the divZ constructor if needed *)
+
+  (* miniACSL arithmetic operation on Z, with the special case of division by zero *)
   Definition arithopZ (op : arithop)(x y : Z) : Z :=
     match op, y with
     | DivOp, 0 => divZ x
@@ -44,24 +46,25 @@ Section operations_definitions2.
     | ModOp, _ => x mod y
     end.
 
-  
+  (*miniACSL unary operation*)
   Inductive tunop :=
   | TNegOp : tunop
   | TComplOp : tunop.
 
+  (*Conversion from miniACSL unary operation to C unary operation*)
   Definition tun_to_un (op : tunop):=
     match op with
     | TNegOp  => NegOp 
     | TComplOp  => ComplOp 
     end.
 
+  (* application of unary operation *)
   Definition tval_unop (op : tunop) (v : val_term K) : val_term K :=
     match v, op with
     | VInteger n, TNegOp => VInteger (-n)
     | ValC v,_ => ValC(val_unop (tun_to_un op) v)
     | _,_ => v
     end.
-
   
   (* New arithop function which takes the divZ constructor when there is a division by zero *)
   Definition new_arithop (op : arithop)(x y : Z) (τi1 τi2 : int_type K) : Z  :=
@@ -71,42 +74,53 @@ Section operations_definitions2.
     end.
 
   (* New operation on int which take divide by zero in account *)
-  Definition new_int_binop (op : arithop) (x1 x2 : Z) (τi1 τi2 : int_type K) : Z :=
-     new_arithop op x1 x2 τi1 τi2
-    .
+  Definition new_int_binop (op : binop) (x1 x2 : Z) (τi1 τi2 : int_type K) : Z :=
+    match op with
+    | ArithOp op => new_arithop op x1 x2 τi1 τi2
+    | _ => int_binop op x1 τi1 x2 τi2
+    end.
   
   (* New operation on base_val which take divide by zero in account *)
   Definition new_base_val_binop (en : env K) (op : binop) (v1 v2 : base_val K): base_val K :=
-    match v1, v2, op with
-    | VInt τi1 x1, VInt τi2 x2, ArithOp aop =>
-        VInt (int_binop_type_of op τi1 τi2) (new_int_binop aop x1 x2 τi1 τi2)
-    |_,_, _ => base_val_binop en op v1 v2
+    match v1, v2 with
+    | VInt τi1 x1, VInt τi2 x2 => VInt (int_binop_type_of op τi1 τi2) (new_int_binop op x1 x2 τi1 τi2)
+    |_,_ => base_val_binop en op v1 v2
     end.
 
-  (* New operation on c values which take divide by zero in account *)
+  (*Predicate to know if two miniACSL values are comparable*)
+  Definition valt_compop_ok (en : env K) (v1 v2 : val_term K) : Prop :=
+    match v1,v2 with
+    | VInteger _, VInteger _ => True
+    | VInteger _, ValC( VBase (VInt _ _)) => True
+    | ValC( VBase (VInt _ _)), VInteger _ => True
+    | ValC(VBase (VPtr _)), ValC (VBase (VPtr _)) => True
+    | ValC(VStruct _ _), ValC(VStruct _ _)=> True
+    | ValC(VUnion _ _ _), ValC( VUnion _ _ _)=> True
+    | ValC(VUnionAll _ _), ValC(VUnionAll _ _) => True
+    | ValC(VUnionAll _ _), ValC( VUnion _ _ _) => True
+    | ValC( VUnion _ _ _) , ValC(VUnionAll _ _) => True
+    | _, _ => False
+    end.
+
+
+  (* New operation on val which take divide by zero in account *)
   Definition new_val_binop (en : env K) (op : binop) (v1 v2 : val K) : val K :=
     match v1, v2 with
     | VBase vb1, VBase vb2 => VBase (new_base_val_binop en op vb1 vb2)
     | _,_ => val_binop en op v1 v2
     end.
-  
+
   (*Last operation to sumup all modifications : arithmetic between C int and acsl integer 
-    (convert
-    to acsl integer) *)
+    (convert to acsl integer) *)
   Definition tval_binop (en : env K) (op : tbinop) (vt1 vt2 : val_term K): val_term K :=
     match vt1,vt2,op with
     | VInteger n1, VInteger n2, TArithOp aop => VInteger (arithopZ aop n1 n2)
     | VInteger n1, ValC (VBase (VInt t n2)), TArithOp aop => VInteger (arithopZ aop n1 n2)
     | ValC (VBase (VInt t n1)), VInteger n2, TArithOp aop => VInteger (arithopZ aop n1 n2)
     | ValC v1, ValC v2, _ => ValC (new_val_binop en (tbin_to_bin op) v1 v2)
-    | VInteger n1, ValC(ptrV p), TArithOp aop => ValC (ptrV (ptr_plus en n1 p))
-    | ValC(ptrV p), VInteger n1, TArithOp aop => ValC (ptrV (ptr_plus en n1 p))
     | _,_,_ => vt1
     end.
 
-
-
-  (* Inductive predicate used to know if a value and a list of values can be compared (predicate used in proofs) *)
   Inductive comparable : val K -> Prop :=
   | cmp_base : forall b, comparable (VBase b)
   | cmp_struct : forall t l, comparable_list l -> comparable (VStruct t l)
@@ -117,96 +131,93 @@ Section operations_definitions2.
   | cmp_nil : comparable_list []
   | cmp_cons : forall v l, comparable v -> comparable_list l -> comparable_list (v::l).
 
-   
-   (* Equality between C values *)
-  Inductive eq_val : env K -> val K -> val K -> mem K -> Prop :=
-  | eq_base : forall(en : env K) (vb1 vb2 : base_val K)(m : mem K),
-      base_val_binop_ok en m (CompOp EqOp) vb1 vb2 ->
+  (* Equality of C values *)
+  Inductive eq_val : env K -> val K -> val K -> Prop :=
+  | eq_base : forall(en : env K) (vb1 vb2 : base_val K),
       new_base_val_binop en (CompOp EqOp) vb1 vb2 = VInt sintT 1 ->
-      eq_val en (VBase vb1) (VBase vb2) m
+      eq_val en (VBase vb1) (VBase vb2)
   | eq_struct : forall (en : env K)
-                      (lval1 lval2 : list (val K)) (tag1 tag2 : tag)(m : mem K),
-      eq_list  en lval1 lval2 m
-      -> eq_val en (VStruct tag1 lval1) (VStruct tag2 lval2) m
-  | eq_union1 : forall (en : env K)(v1 v2 vu1 vu2 : val K)(tag1 tag2 : tag)(n1 n2 : nat)(m : mem K),
+                      (lval1 lval2 : list (val K)) (tag1 tag2 : tag),
+      eq_list  en lval1 lval2 
+      -> eq_val en (VStruct tag1 lval1) (VStruct tag2 lval2)
+  | eq_union1 : forall (en : env K)(v1 v2 vu1 vu2 : val K)(tag1 tag2 : tag)(n1 n2 : nat),
       v1 = VUnion tag1 n1 vu1 ->
       v2 = VUnion tag2 n2 vu2  ->
       val_flatten en v1 = val_flatten en v2 ->
-      eq_val en v1 v2 m
+      eq_val en v1 v2
   | eq_union2 : forall (en : env K) (v1 v2 vu1 : val K)
-                       (tag1 tag2 : tag)(n1 : nat) (lval2 : list (val K))(m : mem K),
+                       (tag1 tag2 : tag)(n1 : nat) (lval2 : list (val K)),
       v1 = VUnion tag1 n1 vu1 ->
       v2 = VUnionAll tag2 lval2 ->
       val_flatten en v1 = val_flatten en v2 ->
-      eq_val en v1 v2 m
+      eq_val en v1 v2
   | eq_union3 : forall (en : env K) (v1 v2 vu2 : val K)
-                       (tag1 tag2 : tag)(n2 : nat) (lval1 : list (val K))(m : mem K),
+                       (tag1 tag2 : tag)(n2 : nat) (lval1 : list (val K)),
       v2 = VUnion tag2 n2 vu2 ->
       v1 = VUnionAll tag1 lval1 ->
       val_flatten en v1 = val_flatten en v2 ->
-      eq_val en v1 v2 m
+      eq_val en v1 v2
   | eq_union4 : forall (en : env K) (v1 v2 : val K)
-                       (tag1 tag2 : tag) (lval1 lval2 : list (val K))( m : mem K),
+                       (tag1 tag2 : tag) (lval1 lval2 : list (val K)),
       v2 = VUnionAll tag2 lval2 ->
       v1 = VUnionAll tag1 lval1 ->
       val_flatten en v1 = val_flatten en v2 ->
-      eq_val en v1 v2 m
-  | eq_same : forall (en : env K)(v1 v2 : val K)(m : mem K),
+      eq_val en v1 v2
+  | eq_same : forall (en : env K)(v1 v2 : val K),
       v1 = v2 ->
-      eq_val en v1 v2 m
-             
-  (* Equality between list of C values *)
-  with eq_list : env K -> list (val K) -> list (val K) -> mem K -> Prop :=
-  | eq_list_empty : forall (en : env K) (m : mem K) ,
-      eq_list  en [] [] m
-  | eq_list_cons : forall (en : env K) (v1 v2 : val K) (lvq1 lvq2: list (val K))(m : mem K),
-      eq_val en v1 v2 m ->
-      eq_list en lvq1 lvq2 m ->
-      eq_list en (v1::lvq1) (v2::lvq2) m
-  | eq_list_same : forall (en : env K) (l : list (val K))(m : mem K),
-      eq_list en l l m.
+      eq_val en v1 v2
+  (* Comparison of list of values *)
+  with eq_list : env K -> list (val K) -> list (val K) -> Prop :=
+  | eq_list_empty : forall (en : env K) ,
+      eq_list  en [] []
+  | eq_list_cons : forall (en : env K) (v1 v2 : val K) (lvq1 lvq2: list (val K)),
+      eq_val en v1 v2 ->
+      eq_list en lvq1 lvq2 ->
+      eq_list en (v1::lvq1) (v2::lvq2)
+  | eq_list_same : forall (en : env K) (l : list (val K)),
+      eq_list en l l.
   
-  (* Comparison of values *)
+  (* Comparison of C values *)
   Inductive comp_val : compop -> env K -> val K -> val K -> Prop :=
-  | eq_value : forall (en : env K)(v1 v2 : val K)(m : mem K),
-      eq_val en v1 v2 m  -> comp_val EqOp en v1 v2
+  | eq_value : forall (en : env K)(v1 v2 : val K),
+      eq_val en v1 v2 -> comp_val EqOp en v1 v2
   | comp_other : forall (op : compop)(en : env K) (v1 v2 : val K),
       new_val_binop en (CompOp op) v1 v2 = VBase (VInt sintT 1) ->
       comp_val op en v1 v2.
 
-  (* Equality between ACSL values *)
-  Inductive eq_valt : env K -> val_term K -> val_term K -> mem K-> Prop :=
-  | eq_valc : forall (en : env K)(v1 v2 : val K)(m : mem K),
-      eq_val en v1 v2 m -> eq_valt en (ValC v1) (ValC v2) m
-  | eq_integer : forall (en : env K) (x y : Z)(m : mem K),
-      x = y -> eq_valt en (VInteger x) (VInteger y) m
-  | eq_integerInt : forall (en : env K) (x y : Z) (t : int_type K)(m : mem K),
-      x = y -> eq_valt en (VInteger x) (ValC (VBase (VInt t y))) m
-  | eq_intInteger : forall (en : env K) (x y : Z) (t : int_type K)(m : mem K),
-      x = y -> eq_valt en (ValC (VBase (VInt t x))) (VInteger y) m
-  | eq_samet : forall (en : env K) (v : val_term K)(m : mem K),
-      eq_valt en v v m.
+  (*Equality of miniACSL values*)
+  Inductive eq_valt : env K -> val_term K -> val_term K -> Prop :=
+  | eq_valc : forall (en : env K)(v1 v2 : val K),
+      eq_val en v1 v2 -> eq_valt en (ValC v1) (ValC v2)
+  | eq_integer : forall (en : env K) (x y : Z),
+      x = y -> eq_valt en (VInteger x) (VInteger y)
+  | eq_integerInt : forall (en : env K) (x y : Z) (t : int_type K),
+      x = y -> eq_valt en (VInteger x) (ValC (VBase (VInt t y)))
+  | eq_intInteger : forall (en : env K) (x y : Z) (t : int_type K),
+      x = y -> eq_valt en (ValC (VBase (VInt t x))) (VInteger y)
+  | eq_samet : forall (en : env K) (v : val_term K),
+      eq_valt en v v.
       
-  (* Comparison of integers *)
+  (*Comparison of integer*)
   Inductive comp_int : compop -> Z -> Z -> Prop :=
   | eq_int : forall (x y: Z) , x = y -> comp_int EqOp x y
   | lt_int : forall (x y : Z), x < y -> comp_int LtOp x y
   | le_int : forall (x y : Z), x <= y -> comp_int LtOp x y.
   
- (* Comparison of ACSL values *)
+ (*Comparison on miniACSL values*)
   Inductive comp_valt : compop -> env K -> val_term K -> val_term K -> Prop :=
+  | eq_valuet : forall (en : env K)(v1 v2 : val_term K),
+      eq_valt en v1 v2 -> comp_valt EqOp en v1 v2
   | comp_valc : forall (en : env K)(v1 v2 : val K)(op : compop),
       comp_val op en v1 v2 -> comp_valt op en (ValC v1) (ValC v2)
-  | eq_valuet : forall (en : env K)(v1 v2 : val_term K)(m : mem K),
-      eq_valt en v1 v2 m -> comp_valt EqOp en v1 v2
   | comp_valInt : forall (en : env K)(x y : Z)(op : compop),
       comp_int op x y -> comp_valt op en (VInteger x) (VInteger y)
-  | comp_intInteger : forall (en : env K)(x y : Z)(op : compop)(ty : int_type K),
-      comp_int op x y -> comp_valt op en (ValC (VBase (VInt ty x))) (VInteger y)
-  | comp_integerInt : forall (en : env K)(x y : Z)(op : compop)(ty : int_type K),
-      comp_int op x y -> comp_valt op en (VInteger x) (ValC (VBase (VInt ty y))). 
+  | comp_valIntInteger : forall (en : env K)(x y : Z)(op : compop) t,
+      comp_int op x y -> comp_valt op en (ValC (VBase (VInt t x))) (VInteger y)
+  | comp_valIntegerInt : forall (en : env K)(x y : Z)(op : compop) t,
+      comp_int op x y -> comp_valt op en (VInteger x) (ValC (VBase (VInt t y))) 
+  .
   
-    
   Lemma comp_valt_test : forall en, ~(comp_valt EqOp en (VInteger 8) (VInteger 0))/\
                                       (comp_valt EqOp en (VInteger (divZ 4)) (VInteger (divZ 4))).
   Proof.
@@ -222,81 +233,7 @@ Section operations_definitions2.
     constructor.
     reflexivity.
   Qed.
-  
-  (* Assume that equality furnished in CH2O is symmetric*)
-  Axiom eq_bval_sym : forall(v1 v2 : base_val K)(en : env K)(m : mem K),
-      base_val_binop_ok en m (CompOp EqOp) v1 v2 ->
-      base_val_binop en (CompOp EqOp) v1 v2 = (intV{sintT} 1)%B ->
-      base_val_binop en (CompOp EqOp) v2 v1 = (intV{sintT} 1)%B.
-  
-
-  (* Proof that equality in CH2O with our modification is symetric *)
-  Lemma eq_val_sym : forall(v1 v2 : base_val K)(en : env K)(m : mem K),
-      base_val_binop_ok en m (CompOp EqOp) v1 v2 ->
-      new_base_val_binop en (CompOp EqOp) v1 v2 = (intV{sintT} 1)%B ->
-      new_base_val_binop en (CompOp EqOp) v2 v1 = (intV{sintT} 1)%B.
-    Proof.
-      intros.
-      destruct v1, v2.
-      all : try unfold base_val_binop_ok in H0. all : try contradiction.
-      unfold new_base_val_binop.
-      unfold new_base_val_binop in H1.
-      apply (eq_bval_sym (intV{i} z) (intV{i0} z0) en m).
-      unfold base_val_binop_ok. assumption.
-      assumption.
-      unfold new_base_val_binop.
-      unfold new_base_val_binop in H1.
-      apply (eq_bval_sym (ptrV p) (ptrV p0) en m). unfold base_val_binop_ok.
-      assumption. assumption.
-    Qed.
-
-
-    
-  (* Assume that equality furnished in CH2O is transitive *)
-    Axiom eq_bval_trans : forall (v1 v2 v3 : base_val K)(en : env K)(m : mem K),
-      base_val_binop_ok en m (CompOp EqOp) v1 v2 ->
-      base_val_binop_ok en m (CompOp EqOp) v2 v3 ->
-      base_val_binop en (CompOp EqOp) v1 v2 = (intV{sintT} 1)%B ->
-      base_val_binop en (CompOp EqOp) v2 v3 = (intV{sintT} 1)%B ->
-      base_val_binop en (CompOp EqOp) v1 v3 = (intV{sintT} 1)%B.
-   
-  (* Proof that equality in CH2O with our modification is transitive *)
-    Lemma eq_val_trans : forall (v1 v2 v3 : base_val K)(en : env K)(m : mem K),
-      base_val_binop_ok en m (CompOp EqOp) v1 v2 ->
-      base_val_binop_ok en m (CompOp EqOp) v2 v3 ->
-      new_base_val_binop en (CompOp EqOp) v1 v2 = (intV{sintT} 1)%B ->
-      new_base_val_binop en (CompOp EqOp) v2 v3 = (intV{sintT} 1)%B ->
-      new_base_val_binop en (CompOp EqOp) v1 v3 = (intV{sintT} 1)%B.
-
-    Proof.
-      intros.
-      destruct v1, v2, v3.
-      all : try unfold base_val_binop_ok in H0, H1. all : try contradiction.
-      unfold new_base_val_binop in H2, H3.
-      unfold new_base_val_binop.
-      apply (eq_bval_trans (intV{i} z) (intV{i0} z0) (intV{i1} z1) en m).
-      all : try unfold base_val_binop_ok. all : try assumption.
-      unfold new_base_val_binop in H2, H3.
-      unfold new_base_val_binop.
-      apply (eq_bval_trans (ptrV p) (ptrV p0) (ptrV p1) en m).
-      all : try unfold base_val_binop_ok.
-      all : try assumption.
-    Qed.
-
-    (*Assume that the comparison condition is symetric*)
-    Axiom eq_base_val_ok_sym : forall en m vb1 vb2,
-      base_val_binop_ok en m (CompOp EqOp) vb1 vb2 -> base_val_binop_ok en m (CompOp EqOp) vb2 vb1.
-    (*Assume that the comparison condtion is transitive*)
-  Axiom eq_base_val_ok_trans : forall en m vb1 vb2 vb3,
-      base_val_binop_ok en m (CompOp EqOp) vb1 vb2 ->
-      base_val_binop_ok en m (CompOp EqOp) vb2 vb3 ->
-      base_val_binop_ok en m (CompOp EqOp) vb1 vb3.
       
-  (* Assume that comparing two C int is equivalent to compare their int part in their 
-abstract representation*)
-  Axiom int_cast_eq : forall (t t2 : int_type K) (en : env K) (x y : Z),
-      new_base_val_binop en (CompOp EqOp) (VInt t x) (VInt t2 y) = (VInt sintT 1) <-> x = y.
-
   Section val_ind.
 
 
@@ -317,9 +254,9 @@ abstract representation*)
       | VBase v => HBase v (* If v is a base, apply HBase *)
       | VStruct t l =>
           (* If it is a struct, do a recusion on the list
-           We need to define the list function internally
-           and not as a joined recursion else termination checker
-           will complain *)
+             We need to define the list function internally
+             and not as a joined recursion else termination checker
+             will complain *)
           let fix val_list_ind l := match l as l' return P (VStruct t l') with
                                     | [] => HStructNil t
                                     | v::l => HStructCons v l t _ (val_ind' v) (val_list_ind l)
@@ -337,31 +274,43 @@ abstract representation*)
                                     end in val_list_ind l
       end.
   End val_ind.
- 
   
-  Scheme eq_val_rec := Induction for eq_val Sort Prop
-      with eq_list_rec := Induction for eq_list Sort Prop.
+  
+  (* Assume that equality in CH2O is symmetric*)
+  Axiom eq_val_sym : forall(v1 v2 : base_val K)(en : env K),
+      new_base_val_binop en (CompOp EqOp) v1 v2 = (intV{sintT} 1)%B ->
+      new_base_val_binop en (CompOp EqOp) v2 v1 = (intV{sintT} 1)%B.
+  
+  (* Assume that equality in CH2O is transitive *)
+  Axiom eq_val_trans : forall (v1 v2 v3 : base_val K)(en : env K),
+      new_base_val_binop en (CompOp EqOp) v1 v2 = (intV{sintT} 1)%B ->
+      new_base_val_binop en (CompOp EqOp) v2 v3 = (intV{sintT} 1)%B ->
+      new_base_val_binop en (CompOp EqOp) v1 v3 = (intV{sintT} 1)%B.
 
-   
-  (* Proof of reflexivity of the equality between ACSL values *)
-  Lemma eq_valt_reflexive v en m : eq_valt en v v m.
+
+  Axiom int_cast_eq : forall (t t2 : int_type K) (en : env K) (x y : Z),
+      new_base_val_binop en (CompOp EqOp) (VInt t x) (VInt t2 y) = (VInt sintT 1) <-> x = y.
+
+  
+  (*Proof that our equality on miniACSL values is reflexive *)
+  Lemma eq_valt_reflexive v en : eq_valt en v v.
   Proof.
     intros.
     apply eq_samet.
   Qed.
   
-  (* Proof of symetry of the equality between C values *)
-Lemma eq_val_symetric : forall(v1 v2 : val K)(en : env K)(m : mem K),
-    eq_val en v1 v2 m -> eq_val en v2 v1 m.
+  Scheme eq_val_rec := Induction for eq_val Sort Prop
+      with eq_list_rec := Induction for eq_list Sort Prop.
+
+  (*Proof that our equality on C values is symmetric *)
+  Lemma eq_val_symmetric : forall(v1 v2 : val K)(en : env K),
+      eq_val en v1 v2 -> eq_val en v2 v1.
   Proof.
-    intros vl vr en m Hp.
+    intros vl vr en.
     apply (eq_val_rec
-             (λ en vl vr m (_:eq_val en vl vr m), eq_val en vr vl m)
-             (λ en ll lr m (_: eq_list en ll lr m ), eq_list en lr ll m)).
-    - intros. apply (eq_base en0 vb2 vb1). apply eq_base_val_ok_sym.
-      assumption.
-      apply (eq_val_sym vb1 vb2 en0 m0).
-      assumption.
+             (λ en vl vr (_:eq_val en vl vr), eq_val en vr vl)
+             (λ en ll lr (_: eq_list en ll lr), eq_list en lr ll)).
+    - intros. apply (eq_base en0 vb2 vb1). apply (eq_val_sym vb1 vb2 en0).
       assumption.
     - intros.  apply (eq_struct en0 lval2 lval1 tag2 tag1). assumption.
     - intros. apply (eq_union1 en0 v2 v1 vu2 vu1 tag2 tag1 n2 n1).
@@ -377,16 +326,14 @@ Lemma eq_val_symetric : forall(v1 v2 : val K)(en : env K)(m : mem K),
     - intros. apply (eq_list_cons).
       assumption. assumption.
     - intros. apply eq_list_same.
-    - intros. assumption.
   Qed.
 
-  
-  (* Proof of symetry between ACSL values *) 
-  Lemma eq_val_term_symetric : forall(v1 v2 : val_term K)(en : env K)(m : mem K),
-      eq_valt en v1 v2 m -> eq_valt en v2 v1 m.
+  (*Proof that our equality on miniACSL values is symmetric*)
+  Lemma eq_valt_symmetric : forall(v1 v2 : val_term K)(en : env K),
+      eq_valt en v1 v2 -> eq_valt en v2 v1.
     intros. inversion H0.
-    apply (eq_valc en v3 v0 m).
-    apply eq_val_symetric.
+    apply eq_valc.
+    apply eq_val_symmetric.
     assumption.
     apply eq_integer.
     symmetry.
@@ -395,29 +342,27 @@ Lemma eq_val_symetric : forall(v1 v2 : val K)(en : env K)(m : mem K),
     apply eq_integerInt. lia.
     apply eq_samet.
   Qed.
-
-
-
-  (* Proof of transitivity of equality between C values*)
-  Lemma eq_val_transitive : forall (v1 v2 v3 : val K) (en : env K)(m : mem K),
-      eq_val en v1 v2 m -> eq_val en v2 v3 m -> eq_val en v1 v3 m.
+  
+  (*Proof that our equality on C values is transitive *)
+  Lemma eq_val_transitive : forall (v1 v2 v3 : val K) (en : env K),
+      eq_val en v1 v2 -> eq_val en v2 v3 -> eq_val en v1 v3. 
   Proof.
-    intros v1 v2 v3 en m H12.
+    intros v1 v2 v3 en H12.
+    
     apply (eq_val_rec
-             (λ en v1 v2 m (_ : eq_val en v1 v2 m), ∀ v3, eq_val en v2 v3 m → eq_val en v1 v3 m)
-             (λ en l1 l2 m (_ : eq_list en l1 l2 m), ∀ l3, eq_list en l2 l3 m → eq_list en l1 l3 m)).
-    - intros en0 vb1 vb2 m2 Hok Hvb12 v3' H23. inversion H23. constructor.
-      apply (eq_base_val_ok_trans en0 m2 vb1 vb2 vb3). assumption. assumption.
-      apply (eq_val_trans vb1 vb2 vb3 en0 m2). assumption. assumption. assumption. assumption.
+             (λ en v1 v2 (_ : eq_val en v1 v2), ∀ v3, eq_val en v2 v3 → eq_val en v1 v3)
+             (λ en l1 l2 (_ : eq_list en l1 l2), ∀ l3, eq_list en l2 l3 → eq_list en l1 l3)).
+    - intros en0 vb1 vb2 Hvb12 v3' H23. inversion H23. constructor.
+      apply (eq_val_trans vb1 vb2 vb3 en0). assumption. assumption.
       discriminate. discriminate. discriminate. discriminate.  rewrite <- H0.
-      apply eq_base. assumption. assumption.
-    - intros en0 lval1 lval2 tag1 tag2 m2 Hl12 IHl v3' H23. inversion H23.
+      apply eq_base. assumption.
+    - intros en0 lval1 lval2 tag1 tag2 Hl12 IHl v3' H23. inversion H23.
       constructor. apply IHl. assumption. discriminate. discriminate. discriminate. discriminate.
       rewrite <- H0. 
       apply eq_struct. assumption.
-    - intros en0 v1' v2' vu1 vu2 tag1 tag2 n1 n2 m2 H1 H2 H12' v3' H23.
+    - intros en0 v1' v2' vu1 vu2 tag1 tag2 n1 n2 H1 H2 H12' v3' H23.
       inversion H23.
-      rewrite -> H2 in H5. discriminate. rewrite -> H2 in H4. discriminate.
+      rewrite -> H2 in H4. discriminate. rewrite -> H2 in H4. discriminate.
       apply (eq_union1 en0 v1' v3' vu1 vu3 tag1 tag3 n1 n3).
       assumption. assumption. rewrite -> H4 in H12'. assumption.
       apply (eq_union2 en0 v1' v3' vu1 tag1 tag3 n1 lval2). assumption. assumption.
@@ -426,8 +371,8 @@ Lemma eq_val_symetric : forall(v1 v2 : val K)(en : env K)(m : mem K),
       rewrite -> H2 in H3. discriminate.
       rewrite <- H0. apply (eq_union1 en0 v1' v2' vu1 vu2 tag1 tag2 n1 n2).
       assumption. assumption. assumption.
-    - intros en0 v1' v2' vu1 tag1 tag2 n1 lval2 m2 H1 H2 H12' v3' H23. inversion H23. 
-      rewrite <- H5 in H2. discriminate.
+    - intros en0 v1' v2' vu1 tag1 tag2 n1 lval2 H1 H2 H12' v3' H23. inversion H23. 
+      rewrite <- H4 in H2. discriminate.
       rewrite <- H4 in H2. discriminate.
       rewrite -> H0 in H2. discriminate.
       rewrite -> H0 in H2. discriminate.
@@ -437,8 +382,8 @@ Lemma eq_val_symetric : forall(v1 v2 : val K)(en : env K)(m : mem K),
       rewrite <- H12' in H4. assumption.
       rewrite <- H0. apply (eq_union2 en0 v1' v2' vu1 tag1 tag2 n1 lval2).
       assumption. assumption. assumption.
-    - intros en0 v1' v2' vu2 tag1 tag2 n2 lval1 m2 H2 H1 H12' v3' H23. inversion H23.
-      rewrite <- H5 in H2. discriminate.
+    - intros en0 v1' v2' vu2 tag1 tag2 n2 lval1 H2 H1 H12' v3' H23. inversion H23.
+      rewrite <- H4 in H2. discriminate.
       rewrite <- H4 in H2. discriminate.
       apply (eq_union3 en0 v1' v3' vu0 tag1 tag3 n0 lval1).
       assumption. assumption. rewrite <- H12' in H4. assumption.
@@ -448,8 +393,8 @@ Lemma eq_val_symetric : forall(v1 v2 : val K)(en : env K)(m : mem K),
       rewrite -> H2 in H3. discriminate.
       rewrite <- H0. apply (eq_union3 en0 v1' v2' vu2 tag1 tag2 n2 lval1 ).
       assumption. assumption. assumption.
-    - intros en0 v1' v2' tag1 tag2 lval1 lval2 m2 H2 H1 H12' v3' H23. inversion H23.
-      rewrite <- H5 in H2. discriminate.
+    - intros en0 v1' v2' tag1 tag2 lval1 lval2 H2 H1 H12' v3' H23. inversion H23.
+      rewrite <- H4 in H2. discriminate.
       rewrite <- H4 in H2. discriminate.
       rewrite -> H0 in H2. discriminate.
       rewrite -> H0 in H2. discriminate.
@@ -459,8 +404,8 @@ Lemma eq_val_symetric : forall(v1 v2 : val K)(en : env K)(m : mem K),
       assumption. assumption. rewrite <- H12' in H4. assumption.
       rewrite <- H0. apply (eq_union4 en0 v1' v2' tag1 tag2 lval1 lval2).
       assumption. assumption. assumption.
-    - intros. inversion H0. rewrite e. rewrite <- H4.
-      apply eq_base. assumption. assumption. rewrite e. rewrite <- H3.
+    - intros. inversion H0. rewrite e. rewrite <- H3.
+      apply eq_base. assumption. rewrite e. rewrite <- H3.
       apply eq_struct. assumption.
       rewrite e. apply (eq_union1 en0 v4 v5 vu1 vu2 tag1 tag2 n1 n2).
       assumption. assumption. assumption.
@@ -472,7 +417,7 @@ Lemma eq_val_symetric : forall(v1 v2 : val K)(en : env K)(m : mem K),
       assumption. assumption. assumption.
       rewrite <- H1. rewrite e. apply eq_same. reflexivity.
     - intros. inversion H0. constructor. constructor.
-    - intros en0 v0 v4 lv1 lv2 m2 H04 IH Hl12 IHl l3 Hv41213.
+    - intros en0 v0 v4 lv1 lv2 H04 IH Hl12 IHl l3 Hv41213.
       inversion Hv41213. constructor.
       apply IH. assumption.
       apply IHl. assumption.
@@ -481,92 +426,114 @@ Lemma eq_val_symetric : forall(v1 v2 : val K)(en : env K)(m : mem K),
     - exact H12.
   Qed.
 
-  
-  (* Proof of transitivity of equality between ACSL values*)
-  Lemma eq_valt_transitive : forall (v1 v2 v3 : val_term K) (en : env K)(m : mem K),
-      eq_valt en v1 v2 m -> eq_valt en v2 v3 m -> eq_valt en v1 v3 m. 
-    intros v1 v2 v3 en m H1 H2.
+(*Proof that our equality on miniACSL values is transitive*)
+  Lemma eq_valt_transitive : forall (v1 v2 v3 : val_term K) (en : env K),
+      valt_compop_ok en v1 v2 -> valt_compop_ok en v2 v3 -> eq_valt en v1 v2 -> eq_valt en v2 v3 -> eq_valt en v1 v3. 
+    intros v1 v2 v3 en H0 H00 H1 H2.
     inversion H1.
     inversion H2.
-    
-    + apply (eq_valc en v0 v6 m).
-      rewrite <- H5 in H9.
-      injection H9.
-      intro.
-      rewrite <- H12 in H0.
-      apply (eq_val_transitive v0 v5 v6).
-      assumption.
-      assumption.
-      
-    + rewrite <- H9 in H5. discriminate.
-    + rewrite <- H9 in H5. discriminate.
-      
-    + rewrite <- H9 in H5. injection H5. intro.
-      destruct H0.
-      destruct vb1. discriminate.
+    + apply eq_valc.
+    rewrite <- H6 in H9.
+    injection H9.
+    intro.
+    rewrite <- H11 in H3.
+    apply (eq_val_transitive v0 v5 v6).
+    assumption.
+    assumption.
+    + rewrite <- H9 in H6. discriminate.
+    + rewrite <- H9 in H6. discriminate.
+    + rewrite <- H9 in H6. injection H6. intro.
+      destruct H3.
+      destruct vb1.
+      unfold new_base_val_binop in H3. unfold base_val_binop in H3.
       discriminate.
-      injection H12. intro. rewrite H14 in H13.
-      apply int_cast_eq in H13.
+      unfold new_base_val_binop in H3. unfold base_val_binop in H3.
+      discriminate.
+      injection H11. intro. rewrite -> H12 in H3.
+      apply int_cast_eq in H3.
       apply eq_intInteger.
       lia.
-      unfold new_base_val_binop in H13.
+      unfold new_base_val_binop in H3.
+      unfold base_val_binop in H3.
       destruct vb2.
-      unfold base_val_binop in H13. all : try discriminate.
-      all : try rewrite -> H12 in H13. all : try discriminate.
-      all : try rewrite H12 in H0. all : try discriminate.
-      rewrite H0. 
+      all: try discriminate.
+      rewrite -> H12 in H11.
+      discriminate.
+      rewrite -> H12 in H11.
+      discriminate.
+      rewrite -> H3 in H11.
+      discriminate.
+      rewrite -> H3 in H11.
+      discriminate.
+      rewrite <- H3 in H11.
+      injection H6.
+      intro.
+      rewrite H11.
       apply eq_intInteger.
       lia.
-      
-    + rewrite H9 in H5.
-      rewrite <- H5.
+    + rewrite H9 in H6.
+      rewrite <- H6.
       constructor.
       assumption.
 
     + destruct H2. discriminate.
       constructor.
       rewrite <- H4 in H1.
-      injection H5.
+      injection H6.
       intro.
       lia.
       apply eq_integerInt.
-      injection H5.
+      injection H6.
       lia.
       discriminate.
-      rewrite <- H5.
+      rewrite <- H6.
       constructor.
       assumption.
-      
     + destruct H2.
-      destruct H2. injection H5. intro. rewrite <- H8 in H7.
+      injection H6.
+      intro.
+      destruct H2. injection H6. intro. rewrite <- H8 in H2.
       destruct vb2.
-      all : try rewrite <- H8 in H2.
-      all : try unfold base_val_binop_ok in H2.
-      all : try contradiction.
+      injection H6.
+      intro.
+      rewrite <- H8 in H00.
+      unfold valt_compop_ok in H00.
+      contradiction.
+      rewrite <- H8 in H00.
+      unfold valt_compop_ok in H00.
+      contradiction.
       constructor.
-      apply int_cast_eq in H7.
+      apply int_cast_eq in H2.
       lia.
-      all : try discriminate.
-      all : try rewrite H2 in H5. all : try discriminate.
-      all : try rewrite H7 in H5. all : try discriminate.
-      rewrite <- H5.
+      rewrite <- H8 in H00.
+      
+      unfold valt_compop_ok in H00.
+      contradiction.
+      rewrite <- H8 in H00.
+      unfold valt_compop_ok in H00.
+      contradiction.
+      discriminate.
+      rewrite H2 in H6. discriminate.
+      rewrite H2 in H6. discriminate.
+      rewrite H8 in H6. discriminate.
+      rewrite H8 in H6. discriminate. rewrite H2 in H6.
+      injection H6. intro. rewrite <- H6.
       constructor.
-      assumption.
-      rewrite <- H4 in H1.
+      lia.
+      discriminate.
+      discriminate.
+      constructor.
+      rewrite <- H5 in H1.
       inversion H1.
+      lia.
+      rewrite <- H6.
       constructor.
       lia.
-      rewrite <- H5.
-      constructor. assumption.
-     
-    + destruct H2. discriminate. injection H5. intro. constructor. lia.
-      injection H5. intro.  constructor. constructor. unfold base_val_binop_ok.
-      unfold int_binop_ok. exact I. 
-      unfold new_base_val_binop. apply (int_cast_eq t t0 en x y0). lia.
-      discriminate. rewrite <- H5. constructor. assumption.
+    + destruct H2. discriminate. injection H6. intro. constructor. lia.
+      injection H6. intro. rewrite H7 in H3. rewrite H2 in H3. constructor. constructor.      
+      unfold new_base_val_binop. apply (int_cast_eq t t0 en x y0). assumption.
+      discriminate. rewrite <- H6. constructor. assumption.
     + assumption.
   Qed.
-
-  
+      
 End operations_definitions2.
-
