core_c/predicate_eval.v
@@ -4,19 +4,21 @@ Require Import List String stringmap.
 Import ListNotations.
 Local Coercion Z.of_nat: nat >-> Z.
 
-(* Predicate to know wether a value is initialized or not *)
+(*Indutive to know wether a list of values is initialized or not*)
 Inductive init_val_list `{Env K} : list (val K) -> Prop :=
 | init_list : forall (lv tlv: list (val K)) (hlv : val K),
     lv = hlv::tlv ->
     init_val hlv ->
     init_val_list lv
 with
+(*Indutive to know wether a list of bits is initialized or not*)
   init_bit_list `{Env K} : list (bit K) -> Prop :=
 |init_bits : forall (lb tlb : list (bit K)) (hlb : bit K)(b : bool)(p : ptr_bit K),
     lb = hlb::tlb ->
     hlb =(BBit b) \/ hlb = BPtr p ->
     init_bit_list tlb ->
     init_bit_list lb
+(*Inductive to know wether a value is initialized or not*)
   with init_val `{Env K} : val K -> Prop :=
 | initVBase : forall (en : Env K) (v : val K) (bt : base_type K) (vb : base_val K),
     v = VBase vb ->
@@ -36,73 +38,122 @@ with
     init_bit_list vecb ->
     init_val v.
 
-(* Evaluation of ACSL predicates : Translatio from predicates to Prop*)
+(*Function to define the validity of a pointer*)
+Definition valid_pointer `{Env K} (en : env K) (p : ptr K) (m : mem K) : Prop :=
+  (ptr_alive' m p) /\
+    match p with
+    | Ptr a =>
+        match (addr_type a) with
+        | TType nty =>
+            ( (0<= (addr_object_offset en a)/char_bits) /\
+                ((addr_object_offset en a) + size_of en nty) <= size_of en (addr_type_object a) )
+        | _ => False
+        end
+    | _ => False
+    end.
+
+(*Function to translate a miniACSL predicate to a Rocq Prop*)
 Fixpoint predicate_to_prop `{Env K} (p : predic K ) (en : env K)
-  (rho : stack K) (rhomap : stringmap (stack K)) (m : mem K) (l : labelname) (labmap : stringmap (mem K)): option Prop :=
+  (rho : stack K) (rhomap : stringmap (stack K)) (m : mem K) (l : labelname) (labmap : stringmap (mem K)): Prop :=
   match p with
-  | PTrue => Some True
-  | PFalse => Some False
+  | PTrue => True
+  | PFalse => False
   | PAt p1 =>  predicate_to_prop p1 en rho rhomap m l labmap
   | PRelOp op t1 t2  => let v1 := term_eval_right t1 en rho rhomap m l labmap in
                         let v2 := term_eval_right t2 en rho rhomap m l labmap in
                         match v1,v2 with
-                        | Some(val1), Some(val2) => Some (comp_valt op en val1 val2) 
-                        | _,_ => None
+                        | Some(val1), Some(val2) => comp_valt op en val1 val2
+                        | _,_ => False
                         end
   | POr p1 p2 =>  let prop1 := predicate_to_prop p1 en rho rhomap m l labmap in
                   let prop2 := predicate_to_prop p2 en rho rhomap m l labmap in
-                  match prop1,prop2 with
-                  | Some p1', Some p2' => Some (p1' \/ p2')
-                  | _,_ => None
-                  end
+                  prop1 \/ prop2
   | PAnd p1 p2 => let prop1 := predicate_to_prop p1 en rho rhomap m l labmap in
                   let prop2 := predicate_to_prop p2 en rho rhomap m l labmap in
-                  match prop1,prop2 with
-                  | Some p1', Some p2' => Some (p1' /\ p2')
-                  | _,_ => None
-                  end
+                   prop1 /\prop2
   | PImpl p1 p2 => let prop1 := predicate_to_prop p1 en rho rhomap m l labmap in
                    let prop2 := predicate_to_prop p2 en rho rhomap m l labmap in
-                   match prop1,prop2 with
-                   | Some p1', Some p2' => Some (p1' -> p2')
-                   | _,_ => None
-                   end
+                   prop1 -> prop2
   | PNot p1 => let prop1 := predicate_to_prop p1 en rho rhomap m l labmap in
-               match prop1 with
-               | Some p1' => Some (~p1')
-               | _ => None
-               end
+               ~prop1 
   | PValid t1 => let v1 := term_eval_right t1 en rho rhomap m l labmap in
                  match v1 with
                  | Some (val1) => match val1 with
-                                  | ValC (VBase (VPtr p)) => match p with
-                                                             | NULL _ => Some False
-                                                             | Ptr a => Some(ptr_alive' m p)
-                                                             | FunPtr _ _ _ => Some True
-                                                      end
-                                  | _ => None
+                                  | ValC (VBase (VPtr p)) => valid_pointer en p m
+                                      
+                                  | _ => False
                                   end
-                 | _ => None
+                 | _ => False
                  end
                    
   (* Initialized *)
   | PInit t1 => let v1 := term_eval_right t1 en rho rhomap m l labmap in
                   match v1 with
                   |Some (val1) => match val1 with
-                                  | ValC (VBase (VPtr p)) => match p with
-                                                      | NULL _ => Some False
+                                  | ValC (VBase (VPtr p)) => valid_pointer en p m /\
+                                                      (match p with
+                                                      | NULL _ => False
                                                       | Ptr a => let vad := m !!{en} a in
                                                                  match vad with
-                                                                 | Some(vaddrok) => Some(init_val vaddrok)
-                                                                 | _ => None
+                                                                 | Some(vaddrok) => init_val vaddrok
+                                                                 | _ => False
                                                                  end
-                                                      | FunPtr _ _ _ => Some True
+                                                      | FunPtr _ _ _ => False
                                                                  
-                                                      end
-                                  | _ => None
+                                                      end)
+                                  | _ => False
                                   end
-                  | None => None
+                  | None => False
                   end
   end.
 
 
+Context `{Env K}.
+
+(*Proof that initialized -> valid*)
+Lemma initImpValid t en rho rhomap l labmap m :
+  predicate_to_prop (PInit t) en rho rhomap m l labmap ->
+  predicate_to_prop (PValid t) en rho rhomap m l labmap.
+Proof.
+  intro.
+  unfold predicate_to_prop in H0.
+  unfold predicate_to_prop.
+  destruct (term_eval_right t en rho rhomap m l labmap).
+  destruct v.
+  destruct v.
+  destruct b.
+  assumption.
+  assumption.
+  assumption.
+  destruct H0.
+  all : assumption.
+  
+Qed.
+
+
+(*Proof that valid -> pointer in proper bounds*)
+Lemma offsetbound2 t a en rho rhomap l labmap m nty :
+  predicate_to_prop (PValid t) en rho rhomap m l labmap /\
+    term_eval_right t en rho rhomap m l labmap = Some (ValC (VBase (VPtr (Ptr a)))) /\
+    addr_type a = TType nty -> 
+  (0<=(addr_object_offset en a)/char_bits) /\
+    ((addr_object_offset en a) + size_of en nty) <= size_of en (addr_type_object a).
+  Proof.
+    intros.
+    destruct H0. destruct H1.
+    unfold predicate_to_prop in H0.
+    destruct (term_eval_right t en rho rhomap m l labmap).
+    destruct v.
+    destruct v.
+    destruct b. discriminate. discriminate.    
+    discriminate.
+    injection H1. intro. unfold valid_pointer in H0. destruct H0. destruct p.
+    discriminate. injection H3.
+    intro.
+    rewrite -> H5 in H4.
+    destruct (addr_type a).
+    injection H2.
+    intro. rewrite <- H6.
+    assumption.
+    all: discriminate.
+  Qed.
