core_c/term_eval.v
@@ -7,54 +7,35 @@ Notation lrval_term K := (ptr K + val_term K)%type.
 Arguments ValC {_} _.
 Arguments VInteger {_} _.
 
-(* Définition of maps to keep track of memory states for every labels crossed *)
+(*Definition of maps used to store memories and stacks at given labels*)
 Definition memmap (K : iType) := stringmap (mem K).
+Definition stackmap (K: iType) := stringmap (stack K).
 
-(* Insertion operation on memory maps *)
 #[global] Instance lmap_insert {K} :
   Insert string (mem K) (memmap K) := λ l m lm,
     <[l:=m]>lm.
-(* Lookup operation on memory maps *)
+
 #[global] Instance lmap_lookup {K} : Lookup string (mem K) (memmap K) :=
   @lookup _ _ (memmap K) _.
 
-
-(* Définition of maps to keep track of stack for every labels crossed *)
-Definition stackmap (K: iType) := stringmap (stack K).
- (* Lookup operation on stack maps *)
 #[global] Instance stackmap_lookup {K} : Lookup string (stack K) (stackmap K) :=
   @lookup _ _ (stackmap K) _.
 
 
-(* Definition of underspecified constructors for invalid memory accesses *)
+
+(* Parameter InvalidMemAccessPtr :forall K, ptr K -> ptr K. *)
+(* Parameter InvalidMemAccessInt :forall K, ptr K -> Z. *)
+(* Parameter InvalidMemAccessCompound : forall K, ptr K  -> list (val K). *)
 Parameter InvalidMemAccessPtr :forall K, ptr K -> ptr K.
 Parameter InvalidMemAccessInt :forall K, ptr K -> Z.
-Parameter InvalidMemAccessCompound : forall K, ptr K  -> list (val K).
-
-(* Definition of underspecified contructors for invalid memory accesses 
-depending on a specific label *)
-Parameter InvalidMemAccessPtrLab :forall K, ptr K -> labelname -> ptr K.
-Parameter InvalidMemAccessIntLab :forall K, ptr K -> labelname -> Z.
-Parameter InvalidMemAccessCompoundLab : forall K, ptr K -> labelname -> list (val K).
-
-(*Definition of underspecified constructors for application of ACSL operations on the NULL pointer
-*)
-Parameter InvalidBlockLen : forall K, ptr K -> Z.
-Parameter InvalidOffset : forall K, ptr K -> Z.
-Parameter InvalidBaseaddr : forall K, ptr K -> ptr K.
+Parameter InvalidMemAccessCompound : forall K, ptr K -> list (val K).
 
 Arguments InvalidMemAccessInt {_} _.
 Arguments InvalidMemAccessPtr {_} _.
 Arguments InvalidMemAccessCompound {_} _.
-Arguments InvalidMemAccessIntLab {_} _.
-Arguments InvalidMemAccessPtrLab {_} _.
-Arguments InvalidMemAccessCompoundLab {_} _.
-Arguments InvalidBlockLen {_} _.
-Arguments InvalidOffset {_} _.
-Arguments InvalidBaseaddr {_} _.
 
-                  
-(* Function that converts an invalid pointer into an underpecified ACSL value *)
+
+(*Function that returns a under-specified term for invalid memory access *)
 Definition convertInvalid `{Env K} (p : ptr K) : val_term K :=
   match p with
   | NULL pt => match pt with
@@ -75,33 +56,11 @@ Definition convertInvalid `{Env K} (p : ptr K) : val_term K :=
   end.
 
 
-(*Function that converts an invalid pointer with specific label into an underspecified ACSL value
- *)
-Definition convertInvalidLab `{Env K} (p : ptr K) (l : labelname): val_term K :=
-  match p with
-  | NULL pt => match pt with
-               | TType (TBase (TInt _)) => VInteger (InvalidMemAccessIntLab p l)
-               | TType (TBase (TPtr _)) => ValC (VBase (VPtr (InvalidMemAccessPtrLab p l)))
-               | TType (TCompound Struct_kind t) => ValC (VStruct t (InvalidMemAccessCompoundLab p l))
-               | TType (TCompound Union_kind t) => ValC (VUnionAll t (InvalidMemAccessCompoundLab p l))
-               | _ => VInteger 0
-               end
-  | Ptr a => match (addr_type a) with
-             | TType (TBase (TInt _)) => VInteger (InvalidMemAccessIntLab p l)
-             | TType (TBase (TPtr _)) => ValC (VBase (VPtr (InvalidMemAccessPtrLab p l)))
-             | TType (TCompound Struct_kind t) => ValC (VStruct t (InvalidMemAccessCompoundLab p l))
-             | TType (TCompound Union_kind t) => ValC (VUnionAll t (InvalidMemAccessCompoundLab p l))
-             | _ => VInteger 0
-             end
-  | _=> VInteger 0
-  end.
-
-(* Function that evaluates ACSL terms *)
+(*Function that evaluates ACSL terms*)
 Fixpoint term_eval `{Env K} (t : term K) (en : env K)
   (rho : stack K) (rhomap : stringmap (stack K))(m : mem K) (l :labelname)
   (labmap : stringmap (mem K)) : option (lrval_term K) :=
   match t with
-  (* Variable *)
   | TVar x  => let rhol :=
                  match l with
                  | "Here" => Some rho
@@ -110,143 +69,141 @@ Fixpoint term_eval `{Env K} (t : term K) (en : env K)
                match rhol with
                | Some sta =>
                    '(o,τ) ← sta !! x;
-                    Some (inl (Ptr (addr_top o τ)))
-               | None => None
-               end
-  (* Value *)
-  | TVal v => Some v
-  (* Conversion from right-value to left-value (address dereference : *t ) *)                 
-  | TRtoL t1 => v ← term_eval t1 en rho rhomap m l labmap ≫= maybe inr;
-  let vc := match v with
-            | ValC v1 => Some v1
+Some (inl (Ptr (addr_top o τ)))
+| None => None
+end
+| TVal v => Some v
+| TRtoL t1 => v ← term_eval t1 en rho rhomap m l labmap ≫= maybe inr;
+let vc := match v with
+          | ValC v1 => Some v1
+          | _ => None
+          end
+in
+match vc with
+| Some v1 =>
+    p ← maybe (VBase ∘ VPtr)  v1;
+guard (ptr_alive' m p);
+Some (inl p)
+| _ => None
+end
+| TRofL t => p ← term_eval t en rho rhomap m l labmap ≫= maybe inl;
+Some (inr (ValC (ptrV p)))
+| TBinOp op t1 t2 =>  v1 ← term_eval t1 en rho rhomap m l labmap ≫= maybe inr;
+v2 ← term_eval t2 en rho rhomap m l labmap ≫= maybe inr;
+Some (inr (tval_binop en op v1 v2))
+     
+| TLoad t => p ← term_eval t en rho rhomap m l labmap ≫= maybe (inl);
+let newmopt := match l with
+               | "Here" => Some m
+               | _ => lmap_lookup l labmap
+               end in
+match newmopt with
+| Some newm =>
+    let pi := match p with
+              | NULL _ => Some (inr (convertInvalid p))
+              | Ptr a => let v :=  newm !!{en} a in
+                         match v with
+                         | Some vc => match vc with
+                                      | VBase(VInt _ x) => Some (inr (VInteger x))
+                                      | _ => Some (inr (ValC vc))
+                                      end
+                         | None => Some (inr (convertInvalid p))
+                         end   
+              | _ => None
+              end
+    in pi
+| None => None
+end
+     
+| TUnOp op t => v ← term_eval t en rho rhomap m l labmap ≫= maybe inr;
+Some (inr (tval_unop op v))
+     
+| TEltL t rs =>  a ← term_eval t en rho rhomap m l labmap ≫= maybe (inl ∘ Ptr);
+guard (addr_strict en a);
+Some (inl (Ptr (addr_elt en rs a)))
+     
+| TEltR t rs => v ← term_eval t en rho rhomap m l labmap ≫= maybe (inr);
+let vc := match v with
+          |ValC v1 => Some v1
+          | _ => None
+          end
+in
+match vc with
+| Some vc' =>
+    v' ← vc' !!{en} rs;
+Some (inr  (ValC v'))
+| _ => None
+end
+
+| TBaseAddr t => v ← term_eval t en rho rhomap m l labmap ≫= maybe inr;
+    let vc := match v with
+              | ValC v1 => Some v1
+              | _ => None      
+              end
+    in
+    match vc with
+    | Some v1 => p ← maybe (VBase ∘ VPtr)  v1;
+    guard (ptr_alive' m p);
+        match p with
+        | Ptr a => Some (inl (Ptr (addr_top (addr_index a)(addr_type_object a))))
+        | NULL t => Some (inl (NULL t))
+        | _ => None
+        end
+    | _ => None
+    end
+
+| TOffset t => v ← term_eval t en rho rhomap m l labmap ≫= maybe inr;
+    let vc := match v with
+              | ValC v1 => Some v1
+              | _ => None
+              end
+    in 
+    match vc with
+    | Some v1 => p ← maybe (VBase ∘ VPtr)  v1;
+    guard (ptr_alive' m p);
+        match p with
+        | Ptr a => Some (inr (ValC(VBase(VInt (IntType Signed ptr_rank)
+                                           ((addr_object_offset en a)/char_bits)))))
+        | NULL _ => Some (inr (ValC (VBase (VInt (IntType Signed ptr_rank)
+                                              0))))
+        | _ => None
+        end
+    | _ => None
+end
+
+| TBlckLen t => v ← term_eval t en rho rhomap m l labmap ≫= maybe inr;
+    let vc := match v with
+              | ValC v1 => Some v1
+              | _ => None
+              end
+    in
+    match vc with
+    | Some v1 => p ← maybe (VBase ∘ VPtr)  v1;
+    guard (ptr_alive' m p);
+        match p with
+            | Ptr a => Some (inr (ValC(VBase (VInt (IntType Signed ptr_rank)
+                                                (size_of en (addr_type_object a))))))
+            | NULL _ => Some (inr (ValC (VBase (VInt (IntType Signed ptr_rank)
+                                                  0))))
             | _ => None
-            end
-  in
-  match vc with
-  | Some v1 =>
-      p ← maybe (VBase ∘ VPtr)  v1;
-      guard (ptr_alive' m p);
-      Some (inl p)
-  | _ => None
-  end
-  (* Conversion from left-value to right-value (address of a term : &t )*)
-  | TRofL t => p ← term_eval t en rho rhomap m l labmap ≫= maybe inl;
-               Some (inr (ValC (ptrV p)))
-  (* Binary operation *)
-  | TBinOp op t1 t2 =>  v1 ← term_eval t1 en rho rhomap m l labmap ≫= maybe inr;
-                        v2 ← term_eval t2 en rho rhomap m l labmap ≫= maybe inr;
-                        Some (inr (tval_binop en op v1 v2))
-  (* Load a value from memory *)
-  | TLoad t => p ← term_eval t en rho rhomap m l labmap ≫= maybe (inl);
-  let newmopt := match l with
-                 | "Here" => Some m
-                 | _ => lmap_lookup l labmap
-                 end in
-  match newmopt with
-  | Some newm =>
-      let pi := match p with
-                | NULL _ => Some (inr (convertInvalid p))
-                | Ptr a => let v :=  newm !!{en} a in
-                           match v with
-                           | Some vc => match vc with
-                                        | VBase(VInt _ x) => Some (inr (VInteger x))
-                                        | _ => Some (inr (ValC vc))
-                                        end
-                           | None => Some (inr (convertInvalid p))
-                           end   
-                | _ => None
-                end
-      in pi
-  | None => Some (inr  (convertInvalidLab p l))
-  end
-  (* Unary operation *)
-  | TUnOp op t => v ← term_eval t en rho rhomap m l labmap ≫= maybe inr;
-                  Some (inr (tval_unop op v))
-  (* Field access as a left-value*)
-  | TEltL t rs =>  a ← term_eval t en rho rhomap m l labmap ≫= maybe (inl ∘ Ptr);
-                   guard (addr_strict en a);
-                   Some (inl (Ptr (addr_elt en rs a)))
-  (* Field access as a right-value*)
-  | TEltR t rs => v ← term_eval t en rho rhomap m l labmap ≫= maybe (inr);
-  let vc := match v with
-            |ValC v1 => Some v1
-            | _ => None
-            end
-  in
-  match vc with
-  | Some vc' =>
-      v' ← vc' !!{en} rs;
-      Some (inr  (ValC v'))
-  | _ => None
-  end
-(* \base_address operation of ACSL*)
-  | TBaseAddr t => v ← term_eval t en rho rhomap m l labmap ≫= maybe inr;
-  let vc := match v with
-            | ValC v1 => Some v1
-            | _ => None      
-            end
-  in
-  match vc with
-  | Some v1 => p ← maybe (VBase ∘ VPtr)  v1;
-  guard (ptr_alive' m p);
-  match p with
-  | Ptr a => Some (inl (Ptr (addr_top (addr_index a)(addr_type_object a))))
-  | NULL _ => Some (inl (InvalidBaseaddr p))
-  | _ => None
-  end
-  | _ => None
-  end
-  (*\offset operation of ACSL*)
-  | TOffset t => v ← term_eval t en rho rhomap m l labmap ≫= maybe inr;
-  let vc := match v with
-            | ValC v1 => Some v1
-            | _ => None
-            end
-  in 
-  match vc with
-  | Some v1 => p ← maybe (VBase ∘ VPtr)  v1;
-  guard (ptr_alive' m p);
-  match p with
-  | Ptr a => Some (inr (ValC(VBase(VInt (IntType Signed ptr_rank)
-                                     ((addr_object_offset en a)/char_bits)))))
-  | NULL _ => Some (inr (ValC (VBase (VInt (IntType Signed ptr_rank)
-                                        (InvalidOffset p )))))
-  | _ => None
-  end
-  | _ => None
-  end
-  (* \block_length operation of ACSL*)
-  | TBlckLen t => v ← term_eval t en rho rhomap m l labmap ≫= maybe inr;
-  let vc := match v with
-            | ValC v1 => Some v1
-            | _ => None
-            end
-  in
-  match vc with
-  | Some v1 => p ← maybe (VBase ∘ VPtr)  v1;
-  guard (ptr_alive' m p);
-  match p with
-  | Ptr a => Some (inr (ValC(VBase (VInt (IntType Signed ptr_rank)
-                                      (size_of en (addr_type_object a))))))
-  | NULL _ => Some (inr (ValC (VBase (VInt (IntType Signed ptr_rank)
-                                        (InvalidBlockLen p)))))
-  | _ => None
-  end
-  | _ => None
-  end
-(*\at operation of ACSL*)
+        end
+    | _ => None
+end
+
 | TAt t lab => term_eval t en rho rhomap m lab labmap
 
 end.
 
-
-
+(*Function to evaluate a term as a right-value*)
 Definition term_eval_right `{Env K} (t: term K) (en : env K)
   (rho : stack K) (rhomap : stringmap (stack K)) (m : mem K)
   (l : labelname) (labmap : stringmap (mem K)) : option(val_term K) :=
   term_eval t en rho rhomap m l labmap ≫= maybe inr.
 
+(*Function to evaluate a term as a left-value*)
 Definition term_eval_left `{Env K} (t: term K) (en : env K)
   (rho : stack K) (rhomap : stringmap (stack K)) (m : mem K)
   (l : labelname) (labmap : stringmap (mem K)) : option (ptr K) :=
   term_eval t en rho rhomap m l labmap ≫= maybe inl.
+
+  
